single-token/USDC/USDC.sol
@@ -49,13 +49,9 @@ library SafeMath {
         return c;
     }
 }
-/**
- * @title FiatToken
- * @dev ERC20 Token backed by fiat reserves
- */
 
-/// @custom:tct invariant: forall x:address :: 0 <= this.balances[x] && this.balances[x] <= this.totalSupply
-/// @custom:tct invariant: sum(this.balances) == this.totalSupply
+/// @custom:tct invariant: forall x:address :: Zero <= this.balances[x] && this.balances[x] <= this.totalSupply
+/// @custom:tct invariant: sum( this.balances ) == this.totalSupply
 contract FiatTokenV1  {
     using SafeMath for uint256;
 
